src/cbor/pulse/CBOR.Pulse.API.Nondet.Rust.fsti
@@ -1,0 +1,422 @@
+module CBOR.Pulse.API.Nondet.Rust
+open CBOR.Spec.Constants
+open Pulse.Lib.Pervasives
+module Spec = CBOR.Spec.API.Format
+module Trade = Pulse.Lib.Trade.Util
+module U8 = FStar.UInt8
+module U64 = FStar.UInt64
+module S = Pulse.Lib.Slice
+module SZ = FStar.SizeT
+module Base = CBOR.Pulse.API.Base
+
+val cbornondet: Type0
+
+noextract [@@noextract_to "krml"]
+val cbor_nondet_match: perm -> cbornondet -> Spec.cbor -> slprop
+
+val cbor_nondet_reset_perm () : Base.reset_perm_t cbor_nondet_match
+
+val cbor_nondet_share () : Base.share_t cbor_nondet_match
+val cbor_nondet_gather () : Base.gather_t cbor_nondet_match
+
+val cbor_nondet_parse (_: unit) : Base.cbor_nondet_parse_t cbor_nondet_match
+
+val cbor_nondet_match_with_size
+  (size: nat)
+  (p: perm)
+  (c: cbornondet)
+  (v: Spec.cbor)
+: Tot slprop
+
+val cbor_nondet_match_with_size_intro (_: unit) : Base.ghost_get_size_t #_ cbor_nondet_match cbor_nondet_match_with_size
+
+val cbor_nondet_size (_: unit) : Base.get_size_t #_ cbor_nondet_match_with_size
+
+val cbor_nondet_serialize
+  (_: unit)
+: Base.cbor_nondet_serialize_t #cbornondet cbor_nondet_match_with_size
+
+(* Constructors *)
+
+noextract [@@noextract_to "krml"]
+let cbor_nondet_mk_simple_value_post
+  (v: U8.t)
+  (res: option cbornondet)
+: Tot slprop
+= match res with
+  | None -> emp
+  | Some res' -> exists* v' . cbor_nondet_match 1.0R res' v' ** pure (simple_value_wf v /\ v' == Spec.pack (Spec.CSimple v))
+
+val cbor_nondet_mk_simple_value
+  (v: U8.t)
+: stt (option cbornondet)
+    emp
+    (fun res ->
+      cbor_nondet_mk_simple_value_post v res **
+      pure (Some? res <==> simple_value_wf v)
+    )
+
+[@@no_auto_projectors]
+type cbor_nondet_int_kind =
+ | UInt64
+ | NegInt64
+
+val cbor_nondet_mk_int64
+  (ty: cbor_nondet_int_kind)
+  (v: U64.t)
+: stt cbornondet
+    emp
+    (fun res -> cbor_nondet_match 1.0R res (Spec.pack (Spec.CInt64 (if ty = UInt64 then cbor_major_type_uint64 else cbor_major_type_neg_int64) v))
+    )
+
+[@@no_auto_projectors]
+type cbor_nondet_string_kind =
+| ByteString
+| TextString
+
+noextract [@@noextract_to "krml"]
+let cbor_nondet_mk_string_post
+  (ty: major_type_byte_string_or_text_string)
+  (s: S.slice U8.t)
+  (p: perm)
+  (v: Seq.seq U8.t)
+  (res: option cbornondet)
+= match res with
+  | None -> pts_to s #p v
+  | Some res' -> exists* v' .
+    cbor_nondet_match 1.0R res' (Spec.pack (Spec.CString ty v')) **
+    Trade.trade
+      (cbor_nondet_match 1.0R res' (Spec.pack (Spec.CString ty v')))
+      (pts_to s #p v) **
+    pure (v' == v)
+
+val cbor_impl_utf8_correct (_: unit) : Base.impl_utf8_correct_t
+
+val cbor_nondet_mk_string
+  (ty: cbor_nondet_string_kind)
+  (s: S.slice U8.t)
+  (#p: perm)
+  (#v: Ghost.erased (Seq.seq U8.t))
+: stt (option cbornondet)
+    (pts_to s #p v)
+    (fun res ->
+      cbor_nondet_mk_string_post (if ty = ByteString then cbor_major_type_byte_string else cbor_major_type_text_string) s p v res **
+      pure (Some? res <==> (FStar.UInt.fits (SZ.v (S.len s)) U64.n /\ (ty == TextString ==> CBOR.Spec.API.UTF8.correct v))) // this is true for Rust's str/String, but we will check anyway
+    )
+
+val cbor_nondet_mk_tagged: Base.mk_tagged_t cbor_nondet_match
+
+val cbor_nondet_map_entry: Type0
+
+noextract [@@noextract_to "krml"]
+val cbor_nondet_map_entry_match: perm -> cbor_nondet_map_entry -> (Spec.cbor & Spec.cbor) -> slprop
+
+val cbor_nondet_mk_map_entry : Base.mk_map_entry_t cbor_nondet_match cbor_nondet_map_entry_match
+
+module PM = Pulse.Lib.SeqMatch
+
+noextract [@@noextract_to "krml"]
+let cbor_nondet_mk_array_post
+  (a: S.slice cbornondet)
+  (pa: perm)
+  (va: (Seq.seq cbornondet))
+  (pv: perm)
+  (vv: (list Spec.cbor))
+  (res: option cbornondet)
+: Tot slprop
+= match res with
+  | None ->
+    pts_to a #pa va **
+    PM.seq_list_match va vv (cbor_nondet_match pv)
+  | Some res ->
+    exists* v' .
+      cbor_nondet_match 1.0R res (Spec.pack (Spec.CArray v')) **
+      Trade.trade
+        (cbor_nondet_match 1.0R res (Spec.pack (Spec.CArray v')))
+        (pts_to a #pa va **
+          PM.seq_list_match va vv (cbor_nondet_match pv)
+        ) **
+        pure (
+          v' == vv
+        )
+
+val cbor_nondet_mk_array
+  (a: S.slice cbornondet)
+  (#pa: perm)
+  (#va: Ghost.erased (Seq.seq cbornondet))
+  (#pv: perm)
+  (#vv: Ghost.erased (list Spec.cbor))
+: stt (option cbornondet)
+    (pts_to a #pa va **
+      PM.seq_list_match va vv (cbor_nondet_match pv)
+    )
+    (fun res ->
+      cbor_nondet_mk_array_post a pa va pv vv res **
+      pure (Some? res <==> FStar.UInt.fits (SZ.v (S.len a)) U64.n)
+    )
+
+val cbor_nondet_mk_map (_: unit): Base.mk_map_gen_t cbor_nondet_match cbor_nondet_map_entry_match
+
+inline_for_extraction
+noextract [@@noextract_to "krml"]
+let cbor_nondet_mk_map_from_array : Base.mk_map_from_array_t cbor_nondet_match cbor_nondet_map_entry_match =
+  Base.mk_map_from_array (CBOR.Pulse.API.Base.mk_map_from_option (cbor_nondet_mk_map ()))
+
+
+(* Destructors *)
+
+val cbor_nondet_equal : Base.equal_t cbor_nondet_match
+
+val cbor_nondet_major_type () : Base.get_major_type_t cbor_nondet_match
+
+noextract [@@noextract_to "krml"]
+let cbor_nondet_tagged_match (p: perm) (tag: U64.t) (payload: cbornondet) (v: Spec.cbor) : Tot slprop =
+  exists* v' .
+    cbor_nondet_match p payload v' **
+    pure (Spec.unpack v == Spec.CTagged tag v')
+
+[@@CAbstractStruct; no_auto_projectors]
+val cbor_nondet_array: Type0
+
+noextract [@@noextract_to "krml"]
+val cbor_nondet_array_match (p: perm) (a: cbor_nondet_array) (v: Spec.cbor) : Tot slprop
+
+[@@CAbstractStruct; no_auto_projectors]
+val cbor_nondet_map: Type0
+
+noextract [@@noextract_to "krml"]
+val cbor_nondet_map_match (p: perm) (a: cbor_nondet_map) (v: Spec.cbor) : Tot slprop
+
+noeq [@@no_auto_projectors]
+type cbor_nondet_view =
+| Int64: (kind: cbor_nondet_int_kind) -> (value: U64.t) -> cbor_nondet_view
+| String: (kind: cbor_nondet_string_kind) -> (payload: S.slice U8.t) -> cbor_nondet_view
+| Array of cbor_nondet_array
+| Map of cbor_nondet_map
+| Tagged: (tag: U64.t) -> (payload: cbornondet) -> cbor_nondet_view
+| SimpleValue of simple_value
+
+noextract [@@noextract_to "krml"]
+let cbor_nondet_string_match (t: major_type_byte_string_or_text_string) (p: perm) (a: S.slice U8.t) (v: Spec.cbor) : Tot slprop =
+  exists* (v': Seq.seq U8.t) .
+    pts_to a #p v' **
+    pure (
+      Spec.CString? (Spec.unpack v) /\ v' == Spec.CString?.v (Spec.unpack v) /\ t == Spec.CString?.typ (Spec.unpack v) /\
+      (t == cbor_major_type_text_string ==> CBOR.Spec.API.UTF8.correct v')
+    )
+
+noextract [@@noextract_to "krml"]
+let cbor_nondet_view_match
+  (p: perm)
+  (x: cbor_nondet_view)
+  (v: Spec.cbor)
+: Tot slprop
+= match x with
+  | Int64 k i -> pure (v == Spec.pack (Spec.CInt64 (if UInt64? k then cbor_major_type_uint64 else cbor_major_type_neg_int64) i))
+  | String k s -> cbor_nondet_string_match (if ByteString? k then cbor_major_type_byte_string else cbor_major_type_text_string)  p s v
+  | Tagged tag pl -> cbor_nondet_tagged_match p tag pl v
+  | Array a -> cbor_nondet_array_match p a v
+  | Map m -> cbor_nondet_map_match p m v
+  | SimpleValue i -> pure (v == Spec.pack (Spec.CSimple i))
+
+noextract [@@noextract_to "krml"]
+let cbor_nondet_destruct_postcond
+  (x: cbor_nondet_view)
+  (v: Spec.cbor)
+: Tot prop
+= match x, Spec.unpack v with
+  | Int64 _ _, Spec.CInt64 _ _
+  | String _ _, Spec.CString _ _
+  | Tagged _ _, Spec.CTagged _ _
+  | Array _, Spec.CArray _
+  | Map _, Spec.CMap _
+  | SimpleValue _, Spec.CSimple _
+  -> True
+  | _ -> False
+
+val cbor_nondet_destruct
+  (c: cbornondet)
+  (#p: perm)
+  (#v: Ghost.erased Spec.cbor)
+: stt cbor_nondet_view
+    (cbor_nondet_match p c v)
+    (fun w -> exists* p' .
+      cbor_nondet_view_match p' w v **
+      Trade.trade
+        (cbor_nondet_view_match p' w v)
+        (cbor_nondet_match p c v) **
+      pure (cbor_nondet_destruct_postcond w v)
+    )
+
+val cbor_nondet_elim_int64 () : Base.elim_int64_t cbor_nondet_match
+
+val cbor_nondet_elim_simple_value () : Base.elim_simple_t cbor_nondet_match
+
+val cbor_nondet_get_array_length
+  (x: cbor_nondet_array)
+  (#p: perm)
+  (#y: Ghost.erased Spec.cbor)
+: stt U64.t
+    (cbor_nondet_array_match p x y)
+    (fun res ->
+      cbor_nondet_array_match p x y ** pure (
+        Base.get_array_length_post y res
+      )
+    )
+
+val cbor_nondet_array_iterator_t: Type0
+
+noextract [@@noextract_to "krml"]
+val cbor_nondet_array_iterator_match: perm -> cbor_nondet_array_iterator_t -> list Spec.cbor -> slprop
+
+val cbor_nondet_array_iterator_start
+  (x: cbor_nondet_array)
+  (#p: perm)
+  (#y: Ghost.erased Spec.cbor)
+: stt cbor_nondet_array_iterator_t
+  (cbor_nondet_array_match p x y)
+  (fun res ->
+    (exists* p' l' .
+      cbor_nondet_array_iterator_match p' res l' **
+      Trade.trade
+        (cbor_nondet_array_iterator_match p' res l')
+        (cbor_nondet_array_match p x y) **
+      pure (
+        Spec.CArray? (Spec.unpack y) /\
+        l' == Spec.CArray?.v (Spec.unpack y)
+    ))
+  )
+
+val cbor_nondet_array_iterator_is_empty  : Base.array_iterator_is_empty_t cbor_nondet_array_iterator_match
+
+val cbor_nondet_array_iterator_next : Base.array_iterator_next_t cbor_nondet_match cbor_nondet_array_iterator_match
+
+val cbor_nondet_array_iterator_share : Base.share_t cbor_nondet_array_iterator_match
+
+val cbor_nondet_array_iterator_gather : Base.gather_t cbor_nondet_array_iterator_match
+
+val cbor_nondet_array_iterator_length: Base.array_iterator_length_t cbor_nondet_array_iterator_match
+
+val cbor_nondet_array_iterator_truncate : Base.array_iterator_truncate_t cbor_nondet_array_iterator_match
+
+noextract [@@noextract_to "krml"]
+let safe_get_array_item_post
+  (x: cbor_nondet_array)
+  (i: U64.t)
+  (p: perm)
+  (y: Spec.cbor)
+  (res: option cbornondet)
+: Tot slprop
+= match res with
+  | None -> cbor_nondet_array_match p x y ** pure (Spec.CArray? (Spec.unpack y) /\ U64.v i >= List.Tot.length (Spec.CArray?.v (Spec.unpack y)))
+  | Some res' -> exists* p' y' .
+    cbor_nondet_match p' res' y' **
+    Trade.trade (cbor_nondet_match p' res' y') (cbor_nondet_array_match p x y) **
+    pure (Base.get_array_item_post i y y')
+
+noextract [@@noextract_to "krml"]
+let cbor_nondet_get_array_item_postcond
+  (i: U64.t)
+  (y: Spec.cbor)
+  (res: option cbornondet)
+: Tot prop
+= Spec.CArray? (Spec.unpack y) /\
+  (Some? res <==> U64.v i < List.Tot.length (Spec.CArray?.v (Spec.unpack y)))
+
+val cbor_nondet_get_array_item
+  (x: cbor_nondet_array)
+  (i: U64.t)
+  (#p: perm)
+  (#y: Ghost.erased Spec.cbor)
+: stt (option cbornondet)
+    (cbor_nondet_array_match p x y)
+    (fun res ->
+      safe_get_array_item_post x i p y res **
+      pure (cbor_nondet_get_array_item_postcond i y res)
+    )
+
+val cbor_nondet_map_length
+  (x: cbor_nondet_map)
+  (#p: perm)
+  (#y: Ghost.erased Spec.cbor)
+: stt U64.t
+    (cbor_nondet_map_match p x y)
+    (fun res ->
+      cbor_nondet_map_match p x y ** pure (
+        Base.get_map_length_post y res
+      )
+    )
+
+val cbor_nondet_map_iterator_t: Type0
+
+noextract [@@noextract_to "krml"]
+val cbor_nondet_map_iterator_match: perm -> cbor_nondet_map_iterator_t -> list (Spec.cbor & Spec.cbor) -> slprop
+
+val cbor_nondet_map_iterator_start
+  (x: cbor_nondet_map)
+  (#p: perm)
+  (#y: Ghost.erased Spec.cbor)
+: stt cbor_nondet_map_iterator_t
+  (cbor_nondet_map_match p x y)
+  (fun res ->
+    (exists* p' l' .
+      cbor_nondet_map_iterator_match p' res l' **
+      Trade.trade
+        (cbor_nondet_map_iterator_match p' res l')
+        (cbor_nondet_map_match p x y) **
+      pure (
+        Base.map_iterator_start_post y l'
+    ))
+  )
+
+val cbor_nondet_map_iterator_is_empty : Base.map_iterator_is_empty_t cbor_nondet_map_iterator_match
+
+val cbor_nondet_map_iterator_next : Base.map_iterator_next_t cbor_nondet_map_entry_match cbor_nondet_map_iterator_match
+
+val cbor_nondet_map_iterator_share : Base.share_t cbor_nondet_map_iterator_match
+
+val cbor_nondet_map_iterator_gather : Base.gather_t cbor_nondet_map_iterator_match
+
+val cbor_nondet_map_entry_key : Base.map_entry_key_t cbor_nondet_map_entry_match cbor_nondet_match
+
+val cbor_nondet_map_entry_value : Base.map_entry_value_t cbor_nondet_map_entry_match cbor_nondet_match
+
+val cbor_nondet_map_entry_share : Base.share_t cbor_nondet_map_entry_match
+
+val cbor_nondet_map_entry_gather : Base.gather_t cbor_nondet_map_entry_match
+
+noextract [@@noextract_to "krml"]
+let safe_map_get_post
+  (x: cbor_nondet_map)
+  (px: perm)
+  (vx: Spec.cbor)
+  (vk: Spec.cbor)
+  (res: option cbornondet)
+: Tot slprop
+= match res with
+  | None ->
+    cbor_nondet_map_match px x vx ** pure (Spec.CMap? (Spec.unpack vx) /\ None? (Spec.cbor_map_get (Spec.CMap?.c (Spec.unpack vx)) vk))
+  | Some x' ->
+    exists* px' vx' .
+      cbor_nondet_match px' x' vx' **
+      Trade.trade
+        (cbor_nondet_match px' x' vx')
+        (cbor_nondet_map_match px x vx) **
+      pure (Spec.CMap? (Spec.unpack vx) /\ Spec.cbor_map_get (Spec.CMap?.c (Spec.unpack vx)) vk == Some vx')  
+
+val cbor_nondet_map_get
+  (x: cbor_nondet_map)
+  (k: cbornondet)
+  (#px: perm)
+  (#vx: Ghost.erased Spec.cbor)
+  (#pk: perm)
+  (#vk: Ghost.erased Spec.cbor)
+: stt (option cbornondet)
+    (cbor_nondet_map_match px x vx ** cbor_nondet_match pk k vk)
+    (fun res ->
+      cbor_nondet_match pk k vk **
+      safe_map_get_post x px vx vk res **
+      pure (Spec.CMap? (Spec.unpack vx) /\ (Some? (Spec.cbor_map_get (Spec.CMap?.c (Spec.unpack vx)) vk) == Some? res))
+    )
+
+val dummy_cbor_nondet_t (_: unit) : cbornondet
